ArchSemTinyArm/Test.lean
@@ -5,13 +5,21 @@ open ArchSem.TerminatingModel
 open ArchSem.LitmusTest
 open ArchSemTinyArm
 
+/-!
+This file contains regression tests for all TinyArm concurrency models.
+-/
+
+-- TODO: add some more tests here for regression. (maybe diy 6-cycle 2-thread tests?)
+
 namespace ArchSemTinyArm.Promising.Test
 
 def fuel : Nat := 10
+def isem : SailM Unit := sailTinyArmIsem
+
 def naiveModel : ComputationalTerminatingModel :=
-  Promising.createNaiveModel sailTinyArmIsem fuel
+  Promising.createNaiveModel isem fuel
 def promiseFirstModel : ComputationalTerminatingModel :=
-  Promising.createPromiseFirstModel sailTinyArmIsem fuel
+  Promising.createPromiseFirstModel isem fuel
 
 #eval guardTestFromFile true naiveModel "litmus_tests/MP.archsem.toml"
 #eval guardTestFromFile true naiveModel "litmus_tests/MP+dmbs.archsem.toml"
