ArchSem/NondeterministicMonad.lean
@@ -164,4 +164,35 @@ def discardNone : Option α → NEStateM σ ε α
 
 end NEStateM
 
+section Lemmas
+
+theorem NExcept.bind_iff {ε α β} (b : β) (m : NExcept ε α) (f : α → NExcept ε β)
+     : b ∈ (NExcept.bind m f).oks ↔ ∃ (a : α), a ∈ m.oks ∧ b ∈ (f a).oks
+  := by
+  simp only [NExcept.bind]
+  induction m.oks with
+  | nil =>
+    apply Iff.intro
+    all_goals simp
+  | cons a tail ih =>
+    simp only [NExcept.merge, List.foldr, List.map, List.mem_append]
+    apply Iff.intro
+    case mp =>
+      rintro (h | h)
+      · simp [h]
+      · simp [ih.mp h]
+    case mpr =>
+      rintro ⟨a, h_in, h_in_ok⟩
+      cases h_in with
+      | head => exact Or.inl h_in_ok
+      | tail _ h_in_tail => exact Or.inr (ih.mpr ⟨a, h_in_tail, h_in_ok⟩)
+
+theorem NEStateM.bind_iff {ε σ α β} (s₀ : σ) (s : σ) (b : β) (m : NEStateM ε σ α) (f : α → NEStateM ε σ β)
+    : (s, b) ∈ (NEStateM.bind m f s₀).oks ↔ ∃ (s' : σ) (a : α), (s', a) ∈ (m s₀).oks ∧ (s, b) ∈ (f a s').oks
+  := by
+  have h_base := @NExcept.bind_iff (σ × ε) (σ × α) (σ × β) (s, b) (m s₀) (fun p => f p.snd p.fst)
+  simp [Bind.bind, NEStateM.bind, h_base]
+
+end Lemmas
+
 end ArchSem.NondeterministicMonad
